CacheLocal.v
@@ -1,21 +1,39 @@
-Require Import DataTypes Coherence Tree.
+Require Import DataTypes Tree.
 
-Module mkCacheLocal (coh: Coherence).
+Set Implicit Arguments.
+
+Section CacheLocal.
+  Variable State: Set.
+
   Record CacheState :=
     {
-      state: Tree -> Addr -> coh.t;
-      dir: Tree -> Tree -> Addr -> coh.t;
+      state: Tree -> Addr -> State;
+      dir: Tree -> Tree -> Addr -> State;
       data: Tree -> Addr -> Data;
       wait: Tree -> Addr -> bool;
-      waitS: Tree -> Addr -> coh.t;
+      waitS: Tree -> Addr -> State;
       dwait: Tree -> Tree -> Addr -> bool;
-      dwaitS: Tree -> Tree -> Addr -> coh.t;
+      dwaitS: Tree -> Tree -> Addr -> State;
       next: Tree -> nat
     }.
 
   Record CacheLocal :=
     {
       getCacheState: Time -> CacheState;
-      respFn: Time -> option Resp
+      respFn: Time -> option Resp;
+      respFnIdx: forall t,
+                   match respFn t with
+                     | Some (Build_Resp c i _) => i = next (getCacheState t) (p_node c)
+                     | None => True
+                   end;
+      respFnLdData: forall t,
+                      match respFn t with
+                        | Some (Build_Resp c _ d) =>
+                          match desc (reqFn c t) with
+                            | Ld => d = data (getCacheState t) (p_node c) (loc (reqFn c t))
+                            | St => d = initData zero
+                          end
+                        | None => True
+                      end
     }.
-End mkCacheLocal.
+End CacheLocal.
